src/Pipit.System.fst
@@ -22,49 +22,86 @@ type stepfun (input: Type) (state: Type) (result: Type) =
   r: result ->
   prop
 
+let system_map2 (#input #state1 #state2 #value1 #value2 #result: Type) (f: value1 -> value2 -> result)
+  (t1: stepfun input state1 value1)
+  (t2: stepfun input state2 value2):
+       stepfun input (state1 * state2) result =
+  (fun i s s' r ->
+     let s1, s2 = match s with
+         | None -> None, None
+         | Some (s1, s2) -> Some s1, Some s2
+     in
+     let s1', s2' = s' in
+     exists (r1: value1) (r2: value2).
+               t1 i s1 s1' r1 /\
+               t2 i s2 s2' r2 /\
+               r == f r1 r2)
+
+let system_pre (#input #state1 #v: Type) (init: v)
+  (t1: stepfun input state1 v):
+       stepfun input (state1 * v) v =
+  (fun i s s' r ->
+      let s1, v = match s with
+      | None -> None, init
+      | Some (s1, v) -> Some s1, v
+      in
+      let s1', v' = s' in
+      t1 i s1 s1' v' /\ r == v)
+
+let system_then (#input #state1 #state2 #v: Type)
+  (t1: stepfun input state1 v)
+  (t2: stepfun input state2 v):
+       stepfun input state2 v =
+  (fun i s s' r ->
+     match s with
+     | None -> exists s1' r'. t1 i None s1' r /\ t2 i None s' r'
+     | Some _ -> t2 i s s' r)
+
+let system_mu (#input #input' #state1 #v: Type)
+  (extend: input -> v -> input')
+  (t1: stepfun input' state1 v):
+       stepfun input state1 v =
+  (fun i s s' r ->
+      t1 (extend i r) s s' r)
+
 (* A system we get from translating an expression *)
 let xsystem (input: nat) (state: Type) = stepfun (C.vector value input) state value
 
-let rec system_of_exp (e: exp) (vars: nat) (#hwf: squash (wf e vars)):
-    state: Type & xsystem vars state =
+
+let rec state_of_exp (e: exp): Type =
   match e with
-  | XVal v ->
-    (| unit, (fun i s s' r -> r == v) |)
-  | XVar x ->
-    (| unit, (fun i s s' r -> r == C.vector_index i x) |)
+  | XVal v -> unit
+  | XVar x -> unit
+  | XPrim2 p e1 e2 -> state_of_exp e1 * state_of_exp e2
+  | XPre e1 -> state_of_exp e1 * value
+  | XThen e1 e2 -> state_of_exp e2
+  | XMu e1 -> state_of_exp e1
+
+unfold
+let explicit_cast (#a: Type) (b: Type { a == b }) (input: a): b = input
+
+let rec system_of_exp (e: exp) (vars: nat { wf e vars }):
+    xsystem vars (state_of_exp e) =
+  match e with
+  | XVal v -> (fun i s s' r -> r == v)
+  | XVar x -> (fun i s s' r -> r == C.vector_index i x)
   | XPrim2 p e1 e2 ->
-    let (| st1, t1 |) = system_of_exp e1 vars in
-    let (| st2, t2 |) = system_of_exp e2 vars in
-    (| st1 * st2, (fun i s (s1', s2') r ->
-       let s1, s2 = match s with
-         | None -> None, None
-         | Some (s1, s2) -> Some s1, Some s2
-       in
-       exists (r1 r2: value).
-             t1 i s1 s1' r1 /\
-             t2 i s2 s2' r2 /\
-             r == eval_prim2 p r1 r2)
-    |)
+    system_map2 (eval_prim2 p) (system_of_exp e1 vars) (system_of_exp e2 vars)
   | XPre e1 ->
-    let (| st1, t1 |) = system_of_exp e1 vars in
-    (| st1 * value, (fun i s (s1', v') r ->
-      let s1, v = match s with
-        | None -> None, xpre_init
-        | Some (s1, v) -> Some s1, v
-      in
-      t1 i s1 s1' v' /\ r == v) |)
+    system_pre xpre_init (system_of_exp e1 vars)
   | XThen e1 e2 ->
-    let (| st1, t1 |) = system_of_exp e1 vars in
-    let (| st2, t2 |) = system_of_exp e2 vars in
-    (| st2, (fun i s s' r ->
-       match s with
-       | None -> exists s1' r'. t1 i None s1' r /\ t2 i None s' r'
-       | Some _ -> t2 i s s' r)
-    |)
+    let t: xsystem vars (state_of_exp e2) =
+      system_then (system_of_exp e1 vars) (system_of_exp e2 vars)
+    in
+    explicit_cast (xsystem vars (state_of_exp e)) t
   | XMu e1 ->
-    let (| st1, t1 |) = system_of_exp e1 (vars + 1) in
-    (| st1, (fun (i: C.vector value vars) s s' r ->
-      t1 (r :: i) s s' r) |)
+    let t: xsystem (vars + 1) (state_of_exp e1) =
+      system_of_exp e1 (vars + 1)
+    in
+    let t': xsystem vars (state_of_exp e1) =
+      system_mu #(C.vector value vars) #(C.vector value (vars + 1)) (fun i v -> v :: i) t
+    in
+    explicit_cast (xsystem vars (state_of_exp e)) t'
 
 let rec stepn
   (#outer #vars: nat)
@@ -83,409 +120,69 @@ let rec stepn
 
 let rec system_of_exp_invariant
   (#outer #vars: nat)
-  (#state: Type)
-  (e: exp)
-  (t: xsystem vars state)
-  (#hwf: squash (wf e vars))
-  (#hsys: squash (system_of_exp e vars == (| state, t|)))
+  (e: exp { wf e vars /\ causal e })
   (streams: C.table (outer + 1) vars)
   (vs: C.vector value (outer + 1))
   (hBS: bigstep streams e vs)
-  (s: state):
-    Tot Type (decreases e) =
+  (s: state_of_exp e):
+    Tot prop (decreases e) =
   match e with
   | XVar _ -> unit
   | XVal _ -> unit
   | XPrim2 _ e1 e2 ->
-    let (| st1, t1 |) = system_of_exp e1 vars in
-    let (| st2, t2 |) = system_of_exp e2 vars in
-    let (s1, s2) = s <: (st1 * st2) in
+    let (s1, s2) = s <: (state_of_exp e1 * state_of_exp e2) in
     let BSPrim2 _ _ _ _ vs1 vs2 hBS1 hBS2 = hBS in
-    system_of_exp_invariant e1 t1 streams vs1 hBS1 s1 *
-    system_of_exp_invariant e2 t2 streams vs2 hBS2 s2
+    system_of_exp_invariant e1 streams vs1 hBS1 s1 /\
+    system_of_exp_invariant e2 streams vs2 hBS2 s2
   | XPre e1 ->
     let BSPre _ _ _ vs1 hBS1 = hBS in
-    let (| st1, t1 |) = system_of_exp e1 vars in
-    let (s1, v) = s <: (st1 * value) in
-    (hBS': bigstep streams e1 (v :: vs1) * unit)
-      // & system_of_exp_invariant #outer #vars e1 t1 streams (v :: vs1) hBS' s1)
+    let v1'   = bigstep_monotone_inv_next #outer #vars #streams hBS1 in
+    let hBS1' = bigstep_monotone_inv #outer #vars #streams hBS1 in
+    let (s1, v1) = s <: (state_of_exp e1 * value) in
+    (system_of_exp_invariant #outer #vars e1 streams (v1' :: vs1) hBS1' s1 /\ v1 == v1')
 
   | XThen e1 e2 ->
-    let (| st1, t1 |) = system_of_exp e1 vars in
-    let (| st2, t2 |) = system_of_exp e2 vars in
-    let s2 = s <: st2 in
+    let s2 = explicit_cast (state_of_exp e2) s in
     let BSThen _ _ _ vs1 vs2 hBS1 hBS2 = hBS in
-    system_of_exp_invariant e2 t2 streams vs2 hBS2 s2
+    system_of_exp_invariant e2 streams vs2 hBS2 s2
   | XMu e1 ->
-    let (| st1, t1 |) = system_of_exp e1 (vars + 1) in
-    let s1 = s <: st1 in
+    let s1 = explicit_cast (state_of_exp e1) s in
     let BSMu _ _ vs1 hBS1 = hBS in
     let hBS' = bigstep_substitute_XMu e1 streams vs hBS in
-    system_of_exp_invariant #outer #(vars + 1) e1 t1 (C.table_map_append (C.table_of_values vs1) streams) vs1 hBS' s1
+    system_of_exp_invariant #outer #(vars + 1) e1 (C.table_map_append (C.table_of_values vs1) streams) vs1 hBS' s1
 
 let rec step0_ok
   (#vars: nat)
-  (#state: Type)
-  (e: exp { causal e })
-  (t: xsystem vars state)
-  (#hwf: squash (wf e vars))
-  (#hsys: squash (system_of_exp e vars == (| state, t|)))
+  (e: exp { causal e /\ wf e vars })
   (row: C.vector value vars)
   (v: value)
   (hBS: bigstep (C.Table [C.Row row]) e [v]):
-    (s': state & squash (t row None s' v) & system_of_exp_invariant #0 e t (C.Table [C.Row row]) [v] hBS s') =
+    Tot (s': state_of_exp e & u: unit { system_of_exp e vars row None s' v /\ system_of_exp_invariant #0 e (C.Table [C.Row row]) [v] hBS s' }) (decreases e) =
+  let streams = (C.Table #1 #vars [C.Row #vars row]) in
   match e with
-  | XVal _ ->
-    (| (), (), () |)
-
-  | XVar x ->
-    (| (), (), () |)
+  | XVal _ -> (| (), () |)
+  | XVar x -> (| (), () |)
 
   | XPrim2 p e1 e2 ->
     let BSPrim2 _ _ _ _ [v1] [v2] hBS1 hBS2 = hBS in
-    let (| st1, t1 |) = system_of_exp e1 vars in
-    let (| st2, t2 |) = system_of_exp e2 vars in
-    let (| s1', _, ei1 |) = step0_ok e1 t1 row v1 hBS1 in
-    let (| s2', _, ei2 |) = step0_ok e2 t2 row v2 hBS2 in
-    (| (s1', s2'), (), (ei1, ei2) |)
+    let (| s1', () |) = step0_ok e1 row v1 hBS1 in
+    let (| s2', () |) = step0_ok e2 row v2 hBS2 in
+    (| (s1', s2'), () |)
 
   | XPre e1 ->
-    begin
-    match hBS with
-    | BSPre _ _ _ [] hBS1 ->
-        let (| v1, hBS1' |) = bigstep_monotone_inv #0 #vars #(C.Table [C.Row row]) hBS1 in
-        let (| st1, t1 |) = system_of_exp e1 vars in
-        let (| s1', _, ei1 |) = step0_ok e1 t1 row v1 hBS1' in
-        let s' = (s1', v1) in
-        assert (
-          system_of_exp_invariant #0 #vars e t (C.Table #1 #vars [C.Row row]) [v] hBS s' ==
-          (hBS': bigstep (C.Table #1 #vars [C.Row row]) e1 [v1] * unit));
-          // (hBS': bigstep (C.Table [C.Row row]) e1 [v1] & system_of_exp_invariant #0 #vars e1 t1 (C.Table [C.Row row]) [v1] hBS' s1'));
-        let h': (hBS': bigstep (C.Table [C.Row row]) e1 [v1] & system_of_exp_invariant #0 #vars e1 t1 (C.Table [C.Row row]) [v1] hBS' s1') =
-          (| hBS1', ei1 |) in
-        let h'': system_of_exp_invariant #0 #vars e t _ [v] hBS s' =
-          ( hBS1', () ) in
-        (| s', (), h'' |)
+    let BSPre _ _ _ [] hBS1 = hBS in
+    let v1 = bigstep_monotone_inv_next #0 #vars #streams hBS1 in
+    let hBS1' = bigstep_monotone_inv #0 #vars #streams hBS1 in
+    let (| s1', () |) = step0_ok e1 row v1 hBS1' in
+    (| (s1', v1), () |)
 
-    | _ -> false_elim ()
-    end
-    // admit ()
+  | XThen e1 e2 ->
+    let BSThen _ _ _ [v1] [v2] hBS1 hBS2 = hBS in
+    let (| s1', () |) = step0_ok e1 row v1 hBS1 in
+    let (| s2', () |) = step0_ok e2 row v2 hBS2 in
+    (| explicit_cast (state_of_exp e) s2', () |)
 
-  // | XPre e1 ->
-  //   let BSPre _ _ _ [] hBS1 = hBS in
-  //   let (| v1, hBS1' |) = bigstep_monotone_inv hBS1 in
-  //   let (| st1, t1 |) = system_of_exp e1 vars in
-  //   let (| s1', _, ei1 |) = step0_ok e1 t1 row v1 hBS1' in
-  //   let streams = C.Table [C.Row row] in
-  //   let ei1' : system_of_exp_invariant #0 #vars e1 t1 streams [v1] hBS1' s1' = ei1 in
-  //   assert (v == xpre_init);
-  //   assert (system_of_exp_invariant #0 #vars (XPre e1) t streams [v] hBS (s1', v1) == (hBS': bigstep streams e1 [v1] & system_of_exp_invariant #0 #vars e1 t1 streams [v1] hBS' s1')) by (FStar.Tactics.compute (); FStar.Tactics.dump "ok");
-  //   let hb = (| hBS1', ei1' |) <: system_of_exp_invariant (XPre e1) t streams [v] hBS (s1', v1) in
-  //   (| (s1', v1), (), (| hBS1', ei1' |) |)
-
-  | _ -> admit ()
-
-
-let rec stepn_ok
-  (#outer #vars: nat)
-  (#state: Type)
-  (e: exp)
-  (t: xsystem vars state)
-  (#hwf: squash (wf e vars))
-  (#hsys: squash (system_of_exp e vars == (| state, t|)))
-  (streams: C.table (outer + 1) vars)
-  (vs: C.vector value (outer + 1))
-  (hBS: bigstep streams e vs):
-    (s': state & squash (stepn e t streams vs s')) =
-  match e, streams, vs with
-  | XVal _, C.Table [r], [v] ->
-    (| (), _ |)
-  | XVal _, C.Table (_ :: streams'), v :: vs' ->
-    let (| u, _ |) = stepn_ok #(outer - 1) e t (C.Table streams') vs' (bigstep_monotone hBS) in
-    (| u, _ |)
-
-  | XVar x, C.Table [r], [v] ->
-    (| (), _ |)
-  | XVar x, C.Table (_ :: streams'), v :: vs' ->
-    let (| u, _ |) = stepn_ok #(outer - 1) e t (C.Table streams') vs' (bigstep_monotone hBS) in (| u, _ |)
-  | XPrim2 p e1 e2, C.Table [r], [v] ->
-    let BSPrim2 _ _ _ _ [r1] [r2] hBS1 hBS2 = hBS in
-    let (| st1, t1 |) = system_of_exp e1 vars in
-    let (| st2, t2 |) = system_of_exp e2 vars in
-    let (| s1', _ |) = stepn_ok e1 t1 streams [r1] hBS1 in
-    let (| s2', _ |) = stepn_ok e2 t2 streams [r2] hBS2 in
-    (| (s1', s2'), _ |)
-
-  | XPrim2 p e1 e2, C.Table (C.Row row :: streams'), v :: vs' ->
-    let BSPrim2 _ _ _ _ vs1 vs2 hBS1 hBS2 = hBS in
-    let (| st1, t1 |) = system_of_exp e1 vars in
-    let (| st2, t2 |) = system_of_exp e2 vars in
-    let (| s, _ |) = stepn_ok #(outer - 1) e t (C.Table streams') vs' (bigstep_monotone hBS) in
-    let (s1, s2) = s <: (st1 * st2) in
-    let (| s1', _ |) = stepn_ok e1 t1 streams vs1 hBS1 in
-    let (| s2', _ |) = stepn_ok e2 t2 streams vs2 hBS2 in
-    assert (stepn #(outer - 1) e1 t1 (C.Table streams') (List.Tot.tl vs1) s1);
-    assert (v == eval_prim2 p (List.Tot.hd vs1) (List.Tot.hd vs2));
-    assert (stepn #(outer - 1) e t (C.Table streams') vs' (s1, s2));
-    assert (t1 row (Some s1) s1' (List.Tot.hd vs1));
-    assert (t2 row (Some s2) s2' (List.Tot.hd vs2));
-    assert (t row (Some s) (s1', s2') v);
-    assert (stepn e t streams vs (s1', s2'));
-    (| (s1', s2'), _ |)
-
-
-  // | XVar _, C.Table (_ :: streams'), v :: vs' -> (| (), _ |)
-  | _ -> admit ()
-  // match streams, vs with
-  // | C.Table [C.Row row], [r], [r'] ->
-  //   step0_ok e t row r r' s' hBS
-  // | C.Table (C.Row row :: streams'), r :: vs_e', r' :: vs_t' ->
-  //   admit ()
-    // eliminate exists (s_mid: state). stepn #(outer - 1) e t (C.Table streams') vs_t' s_mid
-    // returns vs_e == vs_t
-    // with hEx.
-    //   let hBS' = bigstep_monotone hBS in
-    //   let _ = stepn_ok #(outer - 1) e t (C.Table streams') vs_e' vs_t' s_mid hBS' in
-    //   match e with
-    //   | XVal _ -> ()
-    //   | XVar _ -> ()
-    //   | XPrim2 p e1 e2 ->
-    //     assert (vs_e' == vs_t');
-    //     let BSPrim2 _ _ _ _ vs_e1 vs_e2 hBS1 hBS2 = hBS in
-    //     let (| st1, t1 |) = system_of_exp e1 vars in
-    //     let (| st2, t2 |) = system_of_exp e2 vars in
-    //     let (s1, s2)   = s_mid <: (st1 * st2) in
-    //     let (s1', s2') = s' <: (st1 * st2) in
-    //     eliminate exists (r1' r2': value). t1 row (Some s1) s1' r1' /\ t2 row (Some s2) s2' r2' /\ r' == eval_prim2 p r1' r2'
-    //     returns r == r'
-    //     with hEx. begin
-    //          let _ = stepn_ok e1 t1 streams vs_e1 vs_e1 s1' hBS1 in
-    //          let _ = stepn_ok e2 t2 streams vs_e2 vs_e2 s2' hBS2 in
-    //          ()
-    //          end
-    //   | _ -> admit ()
-      //   | XPre e1 -> ()
-      //   | XThen e1 e2 ->
-      //   let BSThen _ _ _ [r1] [r2] hBS1 hBS2 = hBS in
-      //   let (| st1, t1 |) = system_of_exp e1 vars in
-      //   let (| st2, t2 |) = system_of_exp e2 vars in
-      //   eliminate exists (s1': st1) (r2': value). t1 row None s1' r' /\ t2 row None s' r2'
-      //   returns r == r'
-      //   with hEx. begin
-      //        let _ = step0_ok e1 t1 row r1 r' s1' hBS1 in
-      //        ()
-      //        end
-      //   | XMu e1 ->
-      //   let BSMu _ _ [r] hBS1 = hBS in
-      //   let (| st1, t1 |) = system_of_exp e1 (vars + 1) in
-      //   let hBS' = bigstep_recursive_XMu #0 e1 (C.table1 (C.Row row)) [] r r' hBS in
-      //   let _ = step0_ok e1 t1 (r' :: row) r r' s' hBS' in
-      //   ()
-
-
-
-let rec step0_ok
-  (#vars: nat)
-  (#state: Type)
-  (e: exp)
-  (t: xsystem vars state)
-  (#hwf: squash (wf e vars))
-  (#hsys: squash (system_of_exp e vars == (| state, t|)))
-  (row: C.vector value vars)
-  (r: value)
-  (hBS: bigstep (C.table1 (C.Row row)) e (C.vector1 r)):
-   Tot (squash (exists (s': state). t row None s' r)) (decreases e) =
- match e with
- | XVal _ -> ()
- | XVar _ -> ()
- | XPrim2 p e1 e2 ->
-   let BSPrim2 _ _ _ _ [r1] [r2] hBS1 hBS2 = hBS in
-   let (| st1, t1 |) = system_of_exp e1 vars in
-   let (| st2, t2 |) = system_of_exp e2 vars in
-   let _ = step0_ok e1 t1 row r1 hBS1 in
-   let _ = step0_ok e2 t2 row r2 hBS2 in
-
-   eliminate exists (s1' : st1) (s2': st2). t1 row None s1' r1 /\ t2 row None s2' r2 /\ r == eval_prim2 p r1 r2
-   returns _ with hEx.
-     assert (t row None (s1', s2') r)
-
- | XPre e1 ->
-    begin
-   match hBS with
-    | BSPre _ _ _ [] hBS1 ->
-        let (| st1, t1 |) = system_of_exp e1 vars in
-        let _ = step0_ok e1 t1 row r1 hBS1 in
-
-        eliminate exists (s1' : st1). t1 row None s1' r1 /\ r == true
-        returns _ with hEx.
-            assert (t row None s1' r)
-    // | _ -> admit () // false_elim ()
-    end
- | _ -> admit ()
- // | XPre e1 -> ()
- // | XThen e1 e2 ->
- //   let BSThen _ _ _ [r1] [r2] hBS1 hBS2 = hBS in
- //   let (| st1, t1 |) = system_of_exp e1 vars in
- //   let (| st2, t2 |) = system_of_exp e2 vars in
- //   eliminate exists (s1': st1) (r2': value). t1 row None s1' r' /\ t2 row None s' r2'
- //   returns r == r'
- //   with hEx. begin
- //     let _ = step0_ok e1 t1 row r1 r' s1' hBS1 in
- //     ()
- //   end
- // | XMu e1 ->
- //   let BSMu _ _ [r] hBS1 = hBS in
- //   let (| st1, t1 |) = system_of_exp e1 (vars + 1) in
- //   let hBS' = bigstep_recursive_XMu #0 e1 (C.table1 (C.Row row)) [] r r' hBS in
- //   let _ = step0_ok e1 t1 (r' :: row) r r' s' hBS' in
- //   ()
-
-// let rec stepn_ok
-//   (#outer #vars: nat)
-//   (#state: Type)
-//   (e: exp)
-//   (t: xsystem vars state)
-//   (#hwf: squash (wf e vars))
-//   (#hsys: squash (system_of_exp e vars == (| state, t|)))
-//   (streams: C.table (outer + 1) vars)
-//   (vs: C.vector value outer)
-//   (r r': value)
-//   (s': state)
-//   (hBS: bigstep streams e (r :: vs))
-//   (#ht: squash (stepn e t streams (r' :: vs) s')):
-//    Tot (squash (r == r')) =
-//   match streams with
-//   | C.Table [C.Row row] ->
-//     step0_ok e t row r r' s' hBS
-//   | C.Table (C.Row row :: streams') ->
-//     eliminate exists (s_mid: state). stepn #(outer - 1) e t (C.Table streams') vs s_mid
-//     returns r == r'
-//     with hEx.
-//       let hBS' = bigstep_monotone hBS in
-//       let _ = stepn_ok #(outer - 1) e t (C.Table streams') vs_e' vs_t' s_mid hBS' in
-//       match e with
-//       | XVal _ -> ()
-//       | XVar _ -> ()
-//       | XPrim2 p e1 e2 ->
-//         let BSPrim2 _ _ _ _ vs_e1 vs_e2 hBS1 hBS2 = hBS in
-//         let (| st1, t1 |) = system_of_exp e1 vars in
-//         let (| st2, t2 |) = system_of_exp e2 vars in
-//         let (s1, s2)   = s_mid <: (st1 * st2) in
-//         let (s1', s2') = s' <: (st1 * st2) in
-//         eliminate exists (r1' r2': value). t1 row (Some s1) s1' r1' /\ t2 row (Some s2) s2' r2' /\ r' == eval_prim2 p r1' r2'
-//         returns r == r'
-//         with hEx. begin
-//              let _ = stepn_ok e1 t1 streams () r1' s1' hBS1 in
-//              let _ = stepn_ok e2 t2 streams r2 r2' s2' hBS2 in
-//              ()
-//              end
-//       | _ -> admit ()
-//       //   | XPre e1 -> ()
-//       //   | XThen e1 e2 ->
-//       //   let BSThen _ _ _ [r1] [r2] hBS1 hBS2 = hBS in
-//       //   let (| st1, t1 |) = system_of_exp e1 vars in
-//       //   let (| st2, t2 |) = system_of_exp e2 vars in
-//       //   eliminate exists (s1': st1) (r2': value). t1 row None s1' r' /\ t2 row None s' r2'
-//       //   returns r == r'
-//       //   with hEx. begin
-//       //        let _ = step0_ok e1 t1 row r1 r' s1' hBS1 in
-//       //        ()
-//       //        end
-//       //   | XMu e1 ->
-//       //   let BSMu _ _ [r] hBS1 = hBS in
-//       //   let (| st1, t1 |) = system_of_exp e1 (vars + 1) in
-//       //   let hBS' = bigstep_recursive_XMu #0 e1 (C.table1 (C.Row row)) [] r r' hBS in
-//       //   let _ = step0_ok e1 t1 (r' :: row) r r' s' hBS' in
-//       //   ()
-
-let rec stepn_ok
-  (#outer #vars: nat)
-  (#state: Type)
-  (e: exp)
-  (t: xsystem vars state)
-  (#hwf: squash (wf e vars))
-  (#hsys: squash (system_of_exp e vars == (| state, t|)))
-  (streams: C.table (outer + 1) vars)
-  (vs_e vs_t: C.vector value (outer + 1))
-  (s': state)
-  (hBS: bigstep streams e vs_e)
-  (#ht: squash (stepn e t streams vs_t s')):
-   Tot (squash (vs_e == vs_t)) =
-  match streams, vs_e, vs_t with
-  | C.Table [C.Row row], [r], [r'] ->
-    step0_ok e t row r r' s' hBS
-  | C.Table (C.Row row :: streams'), r :: vs_e', r' :: vs_t' ->
-    eliminate exists (s_mid: state). stepn #(outer - 1) e t (C.Table streams') vs_t' s_mid
-    returns vs_e == vs_t
-    with hEx.
-      let hBS' = bigstep_monotone hBS in
-      let _ = stepn_ok #(outer - 1) e t (C.Table streams') vs_e' vs_t' s_mid hBS' in
-      match e with
-      | XVal _ -> ()
-      | XVar _ -> ()
-      | XPrim2 p e1 e2 ->
-        assert (vs_e' == vs_t');
-        let BSPrim2 _ _ _ _ vs_e1 vs_e2 hBS1 hBS2 = hBS in
-        let (| st1, t1 |) = system_of_exp e1 vars in
-        let (| st2, t2 |) = system_of_exp e2 vars in
-        let (s1, s2)   = s_mid <: (st1 * st2) in
-        let (s1', s2') = s' <: (st1 * st2) in
-        eliminate exists (r1' r2': value). t1 row (Some s1) s1' r1' /\ t2 row (Some s2) s2' r2' /\ r' == eval_prim2 p r1' r2'
-        returns r == r'
-        with hEx. begin
-             let _ = stepn_ok e1 t1 streams vs_e1 vs_e1 s1' hBS1 in
-             let _ = stepn_ok e2 t2 streams vs_e2 vs_e2 s2' hBS2 in
-             ()
-             end
-      | _ -> admit ()
-      //   | XPre e1 -> ()
-      //   | XThen e1 e2 ->
-      //   let BSThen _ _ _ [r1] [r2] hBS1 hBS2 = hBS in
-      //   let (| st1, t1 |) = system_of_exp e1 vars in
-      //   let (| st2, t2 |) = system_of_exp e2 vars in
-      //   eliminate exists (s1': st1) (r2': value). t1 row None s1' r' /\ t2 row None s' r2'
-      //   returns r == r'
-      //   with hEx. begin
-      //        let _ = step0_ok e1 t1 row r1 r' s1' hBS1 in
-      //        ()
-      //        end
-      //   | XMu e1 ->
-      //   let BSMu _ _ [r] hBS1 = hBS in
-      //   let (| st1, t1 |) = system_of_exp e1 (vars + 1) in
-      //   let hBS' = bigstep_recursive_XMu #0 e1 (C.table1 (C.Row row)) [] r r' hBS in
-      //   let _ = step0_ok e1 t1 (r' :: row) r r' s' hBS' in
-      //   ()
-
-
- // match e with
- // | XVal _ -> ()
- // | XVar _ -> ()
- // | XPrim2 p e1 e2 ->
- //   let BSPrim2 _ _ _ _ [r1] [r2] hBS1 hBS2 = hBS in
- //   let (| st1, t1 |) = system_of_exp e1 vars in
- //   let (| st2, t2 |) = system_of_exp e2 vars in
- //   let (s1', s2') = s' <: (st1 * st2) in
- //   eliminate exists (r1' r2': value). t1 row None s1' r1' /\ t2 row None s2' r2' /\ r' == eval_prim2 p r1' r2'
- //   returns r == r'
- //   with hEx. begin
- //     let _ = step0_ok e1 t1 row r1 r1' s1' hBS1 in
- //     let _ = step0_ok e2 t2 row r2 r2' s2' hBS2 in
- //     ()
- //   end
- // | XPre e1 -> ()
- // | XThen e1 e2 ->
- //   let BSThen _ _ _ [r1] [r2] hBS1 hBS2 = hBS in
- //   let (| st1, t1 |) = system_of_exp e1 vars in
- //   let (| st2, t2 |) = system_of_exp e2 vars in
- //   eliminate exists (s1': st1) (r2': value). t1 row None s1' r' /\ t2 row None s' r2'
- //   returns r == r'
- //   with hEx. begin
- //     let _ = step0_ok e1 t1 row r1 r' s1' hBS1 in
- //     ()
- //   end
- // | XMu e1 ->
- //   let BSMu _ _ [r] hBS1 = hBS in
- //   let (| st1, t1 |) = system_of_exp e1 (vars + 1) in
- //   let hBS' = bigstep_recursive_XMu #0 e1 (C.table1 (C.Row row)) [] r r' hBS in
- //   let _ = step0_ok e1 t1 (r' :: row) r r' s' hBS' in
- //   ()
+  | XMu e1 ->
+    let hBS' = bigstep_substitute_XMu e1 streams [v] hBS in
+    let (| s1', () |) = step0_ok e1 (v :: row) v hBS' in
+    (| explicit_cast (state_of_exp e) s1', () |)
